theories/algebra/base.v
@@ -1,4 +1,4 @@
-From mathcomp Require Export ssreflect.
+From Coq Require Export ssreflect.
 From iris.prelude Require Export prelude.
 Global Set Bullet Behavior "Strict Subproofs".
 Global Open Scope general_if_scope.
