Makefile
@@ -1,51 +1,26 @@
-# Process flags
-ifeq ($(Y), 1)
-	YFLAG=-y
-endif
+# Build Coq sources according to `_CoqProject`.
 
-# Determine Coq version
-COQ_VERSION=$(shell coqc --version | egrep -o 'version 8.[0-9]' | egrep -o '8.[0-9]')
-COQ_MAKEFILE_FLAGS ?=
-
-ifeq ($(COQ_VERSION), 8.6)
-	COQ_MAKEFILE_FLAGS += -arg -w -arg -notation-overridden,-redundant-canonical-projection
-endif
-
-# Forward most targets to Coq makefile (with some trick to make this phony)
-%: Makefile.coq phony
-	+@make -f Makefile.coq $@
+COQ_MAKEFILE := coq_makefile
+REDIR := $(MAKE) -f Makefile.coq
 
 all: Makefile.coq
-	+@make -f Makefile.coq all
+	+@$(REDIR) $@
+.PHONY: all
 
-clean: Makefile.coq
-	+@make -f Makefile.coq clean
-	find \( -name "*.v.d" -o -name "*.vo" -o -name "*.aux" -o -name "*.cache" -o -name "*.glob" -o -name "*.vio" \) -print -delete
-	rm -f Makefile.coq
+cleanall: Makefile.coq
+	+@$(REDIR) $@
+	@echo CLEAN Makefile.coq Makefile.coq.conf
+	@rm -f Makefile.coq Makefile.coq.conf
+.PHONY: cleanall
 
-# Create Coq Makefile
-Makefile.coq: _CoqProject Makefile
-	@# we want to pass the correct name to coq_makefile or it will be confused.
-	coq_makefile $(COQ_MAKEFILE_FLAGS) -f _CoqProject -o Makefile.coq
-	mv Makefile.coq Makefile.coq.tmp
-	@# The sed script is for Coq 8.5 only, it fixes 'make verify'.
-	@# The awk script fixes 'make uninstall'.
-	sed 's/$$(COQCHK) $$(COQCHKFLAGS) $$(COQLIBS)/$$(COQCHK) $$(COQCHKFLAGS) $$(subst -Q,-R,$$(COQLIBS))/' < Makefile.coq.tmp \
-	  | awk '/^uninstall:/{print "uninstall:";print "\tif [ -d \"$$(DSTROOT)\"$$(COQLIBINSTALL)/iris/ ]; then find \"$$(DSTROOT)\"$$(COQLIBINSTALL)/iris/ -name \"*.vo\" -print -delete; fi";getline;next}1' > Makefile.coq
-	rm Makefile.coq.tmp
+# Enable $(REDIR)
+Makefile.coq Makefile.coq.conf: _CoqProject Makefile
+	+@echo COQ_MAKEFILE
+	+@$(COQ_MAKEFILE) -f _CoqProject -o Makefile.coq
 
-# Install build-dependencies
-build-dep:
-	build/opam-pins.sh < opam.pins
-	opam upgrade $(YFLAG) # it is not nice that we upgrade *all* packages here, but I found no nice way to upgrade only those that we pinned
-	opam pin add coq-iris "$$(pwd)#HEAD" -k git -n -y
-	opam install coq-iris --deps-only $(YFLAG)
-	opam pin remove coq-iris
+# $(REDIR)
+%: Makefile.coq
+	+@$(REDIR) $@
 
-# some fiels that do *not* need to be forwarded to Makefile.coq
-Makefile: ;
-_CoqProject: ;
-
-# Phony targets (i.e. targets that should be run no matter the timestamps of the involved files)
-phony: ;
-.PHONY: all clean phony
+# Don't $(REDIR)
+Makefile _CoqProject: ;
